MicroPolicies/Examples/TL.v
@@ -1,6 +1,7 @@
 
 From mathcomp Require Import ssreflect ssrfun eqtype seq ssrint.
-From CoqUtils Require Import fmap fset word.
+From CoqUtils Require Import word.
+From extructures Require Import fmap fset.
 
 Require Extraction.
 Require extraction.ExtrOcamlString.
@@ -9,7 +10,7 @@ Require Import Intermediate.Machine.
 Require Import Common.Definitions.
 Require Import MicroPolicies.Instance.
 Require Import MicroPolicies.Printer.
-Require Import I2MP.Encode.
+(*Require Import I2MP.Encode.*)
 Require Import I2MP.Linearize.
 
 Require Import MicroPolicies.Utils.
@@ -40,7 +41,37 @@ Definition test_alloc : Intermediate.program :=
     (emptym) (* Pre-allocated buffers *)
     (Some 0). (* Main procedure idtac *)
 
+(*
 Definition test_program_machine := load (encode (linearize test_program)).
 Definition test_alloc_machine := load (encode (linearize test_alloc)).
 
 Extraction "/tmp/tl_test.ml" coqstring_of_state test_program_machine test_alloc_machine stepf.
+ *)
+
+Require Import Transitional S2I.Examples.Helper.
+
+Definition fuel := 1000%nat.
+Definition to_run_i1 := compile_intermediate_and_run test_program fuel.
+Definition to_run_i2 := compile_intermediate_and_run test_alloc fuel.
+
+Set Warnings "-extraction-reserved-identifier".
+Extraction "/tmp/run_intermediate_compiled_test_program.ml" to_run_i1.
+Extraction "/tmp/run_intermediate_compiled_test_alloc.ml" to_run_i2.
+
+Definition to_run1 := compile_and_run_from_intermediate test_program fuel.
+Definition to_run2 := compile_and_run_from_intermediate test_alloc fuel.
+
+Set Warnings "-extraction-reserved-identifier".
+Extraction "/tmp/run_mp_compiled_test_program.ml" to_run1.
+Extraction "/tmp/run_mp_compiled_test_alloc.ml" to_run2.
+
+(*
+Require Import Merged Int32.
+
+Definition to_run_mr := @Merged.compile_and_run_from_source_merged_ex concrete_int_32_mt identity fuel.
+(*
+Definition to_run_mr := @I2MP.Examples.Helper.compile_and_run_and_show_from_source_merged concrete_int_32_mt identity fuel.
+*)
+Set Warnings "-extraction-reserved-identifier".
+Extraction "/tmp/run_merged_compiled_identity.ml" to_run_mr.
+*
