S2I/Examples/Helper.v
@@ -6,14 +6,17 @@ Require Import Intermediate.GlobalEnv.
 Require Import S2I.Compiler.
 Require Export Extraction.Definitions.
 
-Definition compile_and_run (p: Source.program) (fuel: nat) :=
-  match compile_program p with
-  | None => print_error ocaml_int_0
-  | Some compiled_p =>
+
+Definition compile_intermediate_and_run compiled_p fuel := 
     let G := prepare_global_env compiled_p in
     let st := CS.initial_machine_state compiled_p in
     match CS.execN fuel G st with
     | None => print_error ocaml_int_1
     | Some n => print_ocaml_int (z2int n)
-    end
+  end.
+
+Definition compile_and_run (p: Source.program) (fuel: nat) :=
+  match compile_program p with
+  | None => print_error ocaml_int_0
+  | Some compiled_p =>compile_intermediate_and_run compiled_p fuel
   end.
