MicroPolicies/Utils.v
@@ -139,11 +139,11 @@ Module DoNotation.
 Import ssrfun.
 
 Notation "'do!' X <- A ; B" :=
-  (obind (fun X => B) A)
+  (obind (fun X => B) (A))
   (at level 200, X ident, A at level 100, B at level 200).
 
 Notation "'do!' X : T <- A ; B" :=
-  (obind (fun X : T => B) A)
+  (obind (fun X : T => B) (A))
   (at level 200, X ident, A at level 100, B at level 200).
 
 Notation "'do!' 'guard' cond ; rest" :=
